update Centaur branch to match trunk

acl2svn/branches/centaur/history-management.lisp
@@ -1844,6 +1844,7 @@
 ;           in-theory                0 (no name introduced)
 ;           in-arithmetic-theory     0 (no name introduced)
 ;           push-untouchable         0
+;           regenerate-tau-data-base 0 (no name introduced)
 ;           remove-untouchable       0
 ;           reset-prehistory         0
 ;           set-body                 0 (no name introduced)
@@ -1919,6 +1920,7 @@
                               (mutual-recursion (strip-cadrs (cdr form)))
                               ((verify-guards in-theory
                                               in-arithmetic-theory
+                                              regenerate-tau-data-base
                                               push-untouchable
                                               remove-untouchable
                                               reset-prehistory
@@ -1959,6 +1961,7 @@
           (mutual-recursion (strip-cadrs (cddr x)))
           ((verify-guards in-theory
                           in-arithmetic-theory
+                          regenerate-tau-data-base
                           push-untouchable remove-untouchable reset-prehistory
                           set-body table)
            0)
@@ -2771,7 +2774,15 @@
                  PREDEFINED
                  DEFAXIOM-SUPPORTER
                  ATTACHMENT ; see Essay on Defattach re: :ATTACHMENT-DISALLOWED
-                 CLAUSE-PROCESSOR))
+                 CLAUSE-PROCESSOR
+                 TAU-PAIR
+                 POS-IMPLICANTS
+                 NEG-IMPLICANTS
+                 UNEVALABLE-BUT-KNOWN
+                 SIGNATURE-RULES-FORM-1
+                 SIGNATURE-RULES-FORM-2
+                 BIG-SWITCH
+                 ))
 
 ; and these are not created by the introductory event of name (which must have
 ; been a defun or constrain) and hence are left untouched here.
@@ -4901,7 +4912,7 @@
                                 (global-val 'proved-functional-instances-alist
                                             wrld)) 
                         wrld)
-                     wrld))
+                       wrld))
 
 ; We set world global 'skip-proofs-seen or 'redef-seen if ld-skip-proofsp or
 ; ld-redefinition-action (respectively) is non-nil and the world global is not
@@ -4934,6 +4945,7 @@
                                             in-arithmetic-theory
                                             in-theory
                                             push-untouchable
+                                            regenerate-tau-data-base
                                             remove-untouchable
                                             reset-prehistory
                                             set-body
@@ -4970,37 +4982,42 @@
             (wrld4 (if cltl-cmd
                        (put-cltl-command cltl-cmd wrld3
                                          currently-installed-wrld)
-                     wrld3))
+                       wrld3)))
+       (er-let*
+         ((wrld5 (tau-visit-event t ev-type namex
+                                  (tau-auto-modep wrld4)
+                                  (ens state)
+                                  ctx wrld4 state)))
 
 ; WARNING: Do not put down any properties here!  The cltl-command should be the
 ; last property laid down before the call of add-event-landmark.  We rely on
 ; this invariant when looking for 'redefined tuples in
 ; compile-uncompiled-defuns and compile-uncompiled-*1*-defuns.
 
-            (wrld5 (add-event-landmark form ev-type namex wrld4
-                                       (global-val 'boot-strap-flg
-                                                   currently-installed-wrld))))
-       (pprogn
-        (f-put-global 'accumulated-ttree ttree state)
-        (cond
-         ((eq chk-theory-inv-p :protect)
-          (revert-world-on-error
-           (let ((state (set-w 'extension wrld5 state)))
-             (er-progn
-              (chk-theory-invariant1 :install
-                                     (ens state)
-                                     theory-invariant-table
-                                     nil ctx state)
-              (value val)))))
-         (t (let ((state (set-w 'extension wrld5 state)))
-              (cond (chk-theory-inv-p
-                     (er-progn
-                      (chk-theory-invariant1 :install
-                                             (ens state)
-                                             theory-invariant-table
-                                             nil ctx state)
-                      (value val)))
-                    (t (value val)))))))))))
+         (let ((wrld6 (add-event-landmark form ev-type namex wrld5
+                                          (global-val 'boot-strap-flg
+                                                      currently-installed-wrld))))
+           (pprogn
+            (f-put-global 'accumulated-ttree ttree state)
+            (cond
+             ((eq chk-theory-inv-p :protect)
+              (revert-world-on-error
+               (let ((state (set-w 'extension wrld6 state)))
+                 (er-progn
+                  (chk-theory-invariant1 :install
+                                         (ens state)
+                                         theory-invariant-table
+                                         nil ctx state)
+                  (value val)))))
+             (t (let ((state (set-w 'extension wrld6 state)))
+                  (cond (chk-theory-inv-p
+                         (er-progn
+                          (chk-theory-invariant1 :install
+                                                 (ens state)
+                                                 theory-invariant-table
+                                                 nil ctx state)
+                          (value val)))
+                        (t (value val)))))))))))))
 
 (deflabel redundant-events
   :doc
@@ -5080,8 +5097,8 @@
   definitions.  If you try to define the same theory name twice, you
   will get a ``name in use'' error.
 
-  An ~ilc[in-theory] event or ~ilc[defattach] event is never redundant because
-  it doesn't define any name.
+  An ~ilc[in-theory], ~ilc[defattach] or ~ilc[regenerate-tau-data-base] event
+  is never redundant because it doesn't define any name.
 
   A ~ilc[push-untouchable] event is redundant if every name supplied is
   already a member of the corresponding list of untouchable symbols.
@@ -5100,10 +5117,17 @@
   it sets an entire table (using keyword ~c[:clear]) to its existing value;
   ~pl[table].
 
-  An ~ilc[encapsulate] event is redundant if and only if a syntactically
-  identical ~ilc[encapsulate] has already been executed under the same
-  ~ilc[default-defun-mode], ~ilc[default-ruler-extenders], and
-  ~ilc[default-verify-guards-eagerness].
+  In most cases, an ~ilc[encapsulate] event is redundant if and only if a
+  syntactically identical ~ilc[encapsulate] has already been executed under the
+  same ~ilc[default-defun-mode], ~ilc[default-ruler-extenders], and
+  ~ilc[default-verify-guards-eagerness].  There are two rather obscure
+  exceptions to this rule.  One exception is relevant only if ~ilc[make-event]
+  is invoked in the earlier ~c[encapsulate]; in that case, it suffices that the
+  two ~c[encapsulate]s are equal after replacing each top-level sub-event of
+  the earlier ~c[encapsulate] by its ~ilc[make-event] expansion.  The other
+  exception is in the case of redefinition (~pl[ld-redefinition-action]), in
+  which case an attempt is made to ignore an earlier ~c[encapsulate] that has
+  already been superseded by redefinition.
 
   An ~ilc[include-book] is redundant if the book has already been included.
 
@@ -5165,10 +5189,10 @@
   names that will not shift around when the ~il[books] are included.  The
   best such names are those created by ~ilc[deflabel].
 
-  ~em[Note About Unfortunate Redundancies:]
+  ~em[Note About Unfortunate Redundancies.]
 
   Notice that our syntactic criterion for redundancy of ~ilc[defun] ~il[events]
-  does not allow redefinition to take effect unless there is a syntactic change
+  may not allow redefinition to take effect unless there is a syntactic change
   in the definition.  The following example shows how an attempt to redefine a
   function can fail to make any change.
   ~bv[]
@@ -5176,18 +5200,46 @@
   (defmacro mac (x) x)
   (defun foo (x) (mac x))
   (defmacro mac (x) (list 'car x))
+  (set-ld-redefinition-action nil state)
   (defun foo (x) (mac x)) ; redundant, unfortunately; foo does not change
   (thm (equal (foo 3) 3)) ; succeeds, showing that redef of foo didn't happen
   ~ev[]
-  The call of macro ~c[mac] was expanded away when the first definition of
-  ~c[foo] was processed, so the new definition of ~c[mac] is not seen in
-  ~c[foo] unless ~c[foo] is redefined; yet our attempt at redefinition failed!
-  An easy workaround is first to supply a different definition of ~c[foo], just
-  before the last definition of ~c[foo] above.  Then that final definition will
-  no longer be redundant.
+  The call of macro ~c[mac] was expanded away before storing the first
+  definition of ~c[foo] for the theorem prover.  Therefore, the new definition
+  of ~c[mac] does not affect the expansion of ~c[foo] by the theorem prover,
+  because the new definition of ~c[foo] is ignored.
 
-  The phenomenon illustrated above can occur even without macros.  Here is a
-  more complex example, based on one supplied by Grant Passmore.
+  One workaround is first to supply a different definition of ~c[foo], just
+  before the last definition of ~c[foo] above.  Then that final definition will
+  no longer be redundant.  However, as a courtesy to users, we strengthen the
+  redundancy check for function definitions when redefinition is active.  If in
+  the example above we remove the form
+  ~c[(set-ld-redefinition-action nil state)], then the problem goes away:
+
+  ~bv[]
+  (set-ld-redefinition-action '(:warn . :overwrite) state)
+  (defmacro mac (x) x)
+  (defun foo (x) (mac x))
+  (defmacro mac (x) (list 'car x))
+  (defun foo (x) (mac x)) ; no longer redundant
+  (thm (equal (foo 3) 3)) ; fails, as we would like
+  ~ev[]
+
+  To summarize: If a ~ilc[defun] form is submitted that meets the usual
+  redundancy criteria, then it may be considered redundant even if a macro
+  called in the definition has since been redefined.  The analogous problem
+  applie to constants, i.e., symbols defined by ~ilc[defconst] that occur in
+  the definition body.  However, if redefinition is currently active the
+  problem goes away: that is, the redundancy check is strengthened to check the
+  ``translated'' body, in which macro calls and constants defined by
+  ~ilc[defconst] are expanded away.
+
+  The above discussion for ~ilc[defun] forms applies to ~ilc[defconst] forms as
+  well.  However, for ~ilc[defmacro] forms ACL2 always checks translated
+  bodies, so such bogus redundancy does not occur.
+
+  Here is more complex example illustrating the limits of redefinition, based
+  on one supplied by Grant Passmore.
   ~bv[]
   (defun n3 () 0)
   (defun n4 () 1)
@@ -5195,51 +5247,48 @@
   (thm (equal (n5) nil)) ; succeeds, trivially
   (set-ld-redefinition-action '(:warn . :overwrite) state)
   (defun n3 () 2)
+  (thm (equal (n5) nil)) ; still succeeds, sadly
   ~ev[]
-  If now we execute ~c[(thm (equal (n5) nil))], it still succeeds even though
-  we expect ~c[(n5)] = ~c[(> (n3) (n4))] = ~c[(> 2 1)] = ~c[t].  That is
-  because the body of ~c[n5] was normalized to ~c[nil].  (Such normalization
-  can be avoided; see the brief discussion of ~c[:normalize] in the
-  documentation for ~ilc[defun].)  So, given this unfortunate situation, one
-  might expect at this point simply to redefine ~c[n5] using the same
-  definition as before, in order to pick up the new definition of ~c[n3].  Such
-  ``redefinition'' would, however, be redundant, for the same reason as in the
-  previous example:  no syntactic change was made to the definition.  The same
-  workaround applies as before: redefine ~c[n5] to be something different, and
-  then redefine ~c[n5] again to be as desired.
+  We may expect the final ~ilc[thm] call to fail because of the following
+  reasoning: ~c[(n5)] = ~c[(> (n3) (n4))] = ~c[(> 2 1)] = ~c[t].  Unfortunatly,
+  the body of ~c[n5] was simplified (``normalized'') to ~c[nil] when ~c[n5] was
+  admitted, so the redefinition of ~c[n3] is ignored during the final ~c[thm]
+  call.  (Such normalization can be avoided; see the brief discussion of
+  ~c[:normalize] in the documentation for ~ilc[defun].)  So, given this
+  unfortunate situation, one might expect at this point simply to redefine
+  ~c[n5] using the same definition as before, in order to pick up the new
+  definition of ~c[n3].  Such ``redefinition'' would, however, be redundant,
+  for the same reason as in the previous example: no syntactic change was made
+  to the definition.  Even with redefinition active, there is no change in the
+  body of ~c[n5], even with macros and constants (defined by ~ilc[defconst])
+  expanded; there are none such!  The same workaround applies as before:
+  redefine ~c[n5] to be something different, and then redefine ~c[n5] again to
+  be as desired.
 
   A related phenomenon can occur for ~ilc[encapsulate].  As explained above, an
   ~c[encapsulate] event is redundant if it is identical to one already in the
   database.  Consider then the following contrived example.
   ~bv[]
-  (encapsulate () (defun foo (x) x))
+  (defmacro mac (x) x)
+  (encapsulate () (defun foo (x) (mac x)))
   (set-ld-redefinition-action '(:warn . :overwrite) state)
-  (defun foo (x) (cons x x))
-  (encapsulate () (defun foo (x) x)) ; redundant!
+  (defmacro mac (x) (list 'car x))
+  (encapsulate () (defun foo (x) (mac x)))
   ~ev[]
   The last ~c[encapsulate] event is redundant because it meets the criterion
-  for redundancy: it is identical to the earlier ~c[encapsulate] event.  A
-  workaround can be to add something trivial to the ~c[encapsulate], for
+  for redundancy: it is identical to the earlier ~c[encapsulate] event.  Even
+  though redefinition is active, and hence ACL2 ``should'' be able to see that
+  the new ~ilc[defun] of ~c[foo] is not truly redundant, nevertheless the
+  criterion for redundancy of ~ilc[encapsulate] allows the new ~c[encapsulate]
+  form to be redundant.
+
+  A workaround can be to add something trivial to the ~c[encapsulate], for
   example:
   ~bv[]
   (encapsulate () 
     (deflabel try2) ; ``Increment'' to try3 next time, and so on.
     (defun foo (x) x))
-  ~ev[]
-
-  The examples above are suggestive but by no means exhaustive.  Consider the
-  following example.
-  ~bv[]
-  (defstub f1 () => *)
-  (set-ld-redefinition-action '(:warn . :overwrite) state)
-  (defun f1 () 3)
-  (defstub f1 () => *) ; redundant -- has no effect
-  ~ev[]
-  The reason that the final ~ilc[defstub] is redundant is that ~c[defstub] is
-  a macro that expands to a call of ~c[encapsulate]; so this is very similar to
-  the immediately preceding example.
-
-  ")
+  ~ev[]")
 
 (defun stop-redundant-event (ctx state)
   (let ((chan (proofs-co state)))
@@ -6180,7 +6229,7 @@
     ((defconst defpkg)
      (zap-doc-string-from-event-form/third-arg form))
     ((verify-guards in-theory
-                    in-arithmetic-theory
+                    in-arithmetic-theory regenerate-tau-data-base
                     push-untouchable remove-untouchable reset-prehistory
                     table encapsulate defstobj) form)
     (otherwise form)))
@@ -13777,45 +13826,6 @@
          (translate-hands-off-hint1@par (list arg) ctx wrld state))
         (t (translate-hands-off-hint1@par arg ctx wrld state))))
 
-; The next few functions are used to produced the formulas represented by
-; type-prescriptions.
-
-(defun convert-returned-vars-to-term-lst (term vars)
-  (cond ((null vars) nil)
-        (t (cons (mcons-term* 'equal term (car vars))
-                 (convert-returned-vars-to-term-lst term (cdr vars))))))
-
-(defun implicate (t1 t2)
-
-; We return a term equivalent to (IMPLIES t1 t2).
-
-  (cond ((equal t1 *t*) t2)
-        ((equal t1 *nil*) *t*)
-        ((equal t2 *t*) *t*)
-        ((equal t2 *nil*) (dumb-negate-lit t1))
-        (t (mcons-term* 'implies t1 t2))))
-
-(defun convert-type-prescription-to-term (tp ens wrld)
-
-; Tp is a type-prescription.  We generate a term that expresses it relative to
-; the supplied ens.  We will usually store this term in the :corollary of tp
-; itself; generally the current :corollary field of tp is *t* right now because
-; tp was generated by putprop-initial-type-prescriptions.  We return
-; the generated corollary term and a ttree citing the type-set-inverter
-; rules used.
-
-  (mv-let (concl ttree)
-          (convert-type-set-to-term (access type-prescription tp :term)
-                                    (access type-prescription tp :basic-ts)
-                                    ens wrld nil)
-          (mv (implicate (conjoin (access type-prescription tp :hyps))
-                         (disjoin
-                          (cons concl
-                                (convert-returned-vars-to-term-lst
-                                 (access type-prescription tp :term)
-                                 (access type-prescription tp :vars)))))
-              ttree)))
-
 (defun truncated-class (rune mapping-pairs classes)
 
 ; Rune is a rune and mapping-pairs and classes are the corresponding
@@ -16778,11 +16788,6 @@
             more-doc-state             ;;; for proof-checker :more command
             pc-ss-alist                ;;; for saves under :instructions hints
             last-step-limit            ;;; propagate step-limit past expansion
-
-; Note that tainted-okp is deliberately omitted from this list of exceptions,
-; since its global value is the one that should be used during event
-; processing.
-
             ))))
     val))
 
@@ -21433,6 +21438,10 @@
            (declare (ignore col))
            (value ':invisible)))
 
+(defrec certify-book-info
+  (full-book-name . other-info)
+  nil) ; could replace with t sometime
+
 (defun active-book-name (wrld state)
 
 ; This returns the full book name (an absolute pathname ending in .lisp) of the
@@ -21441,7 +21450,7 @@
 
   (or (car (global-val 'include-book-path wrld))
       (let ((x (f-get-global 'certify-book-info state)))
-        (cond (x (let ((y (if (consp x) (car x) x)))
+        (cond (x (let ((y (access certify-book-info x :full-book-name)))
                    (assert$ (stringp y) y)))))))
 
 (defrec deferred-ttag-note
